src/util/extset.v
@@ -1,9 +1,9 @@
-Require Export ErrorMonad.
 Require Import extmap.
 From ExtLib Require Import Monads.
-Import MonadNotation.
-
+Require Export Monads.
+Import MonadNotations.
 Local Open Scope monad_scope.
+
 
 (*Slightly different than OCaml: doesnt depend on map*)
 Module Type S.
@@ -93,11 +93,14 @@ Definition partition f s := @M.partition unit (fun e _ => f e) s.
 Definition cardinal := @M.cardinal unit.
 Definition elements := @M.keys unit.
 Definition min_elt (s: t) : errorM elt :=
-  err_bnd (fun y => err_ret (fst y)) (M.min_binding s).
+  y <-- M.min_binding s ;;
+  err_ret (fst y).
 Definition max_elt (s: t) : errorM elt :=
-  err_bnd (fun y => err_ret (fst y)) (M.max_binding s).
+  y <-- M.max_binding s ;;
+  err_ret (fst y).
 Definition choose (s: t) : errorM elt :=
-  err_bnd (fun y => err_ret (fst y)) (@M.choose unit s).
+  y <-- M.choose s ;;
+  err_ret (fst y).
 Definition change (f: bool -> bool) (x: elt) (s: t) : t :=
   M.change (fun a => is_true_o (f (isSome a))) x s.
 Definition union := @M.set_union unit.
